Add read-only section support for ELF AArch64
This patch adds support for reading the read-only section of ELF (AArch64)
and using it.

This is achieved by extending the ELF loader to
(1) find the .rodata section and read it
(2) read the symbol table and find the objects that are defined in `.rodata`
(3) read the relocation info to record which instructions must be updated when loading it.

For ELF AArch64, GCC is typically using `adrp` + `add` combination (which is also
equivalent to the `adrl` pseudoinstruction) to add the PC-relative offset
and correctly find the symbol address.

When relocation is involved, the machine-code isn't just a list of bytes, but
in fact a function that takes the virtual addresses of the symbols and returns the
correct, 'patched' machine code (which is a byte list).
`define_assert_relocs_from_elf` returns that, as well as a list of new definitions
describing the contents of constant data.

This patch also includes `arm/tutorial/symtab_rodata.ml`, which is an example that loads
constant data.

I found that the following references were helpful:
- https://github.com/ARM-software/abi-aa/blob/main/aaelf64/aaelf64.rst#5733relocation-operations
  for overall meanings of AArch64-specific relocations
- https://refspecs.linuxbase.org/elf/gabi4+/ for the structure of an ELF file
- https://github.com/lattera/glibc/blob/master/elf/elf.h#L2731 for kinds of relocations

arm/proofs/arm.ml
@@ -1159,3 +1159,45 @@ let BL_TARGET_CONV =
 let BL_TARGET_TAC =
   ASSUM_LIST (CONV_TAC o CHANGED_CONV o ONCE_DEPTH_CONV o BL_TARGET_CONV) THEN
   REWRITE_TAC [];;
+
+(* ------------------------------------------------------------------------- *)
+(* Handling PC-relative offsets (ADRP + ADD, which is ADRL pseudo-instr)     *)
+(* ------------------------------------------------------------------------- *)
+
+let adrp_within_bounds = new_definition (
+  `adrp_within_bounds (x:int64) (pc:int64) =
+    let xhi = word_subword x (12,54):(54)word in
+    let pchi = word_subword pc (12,54):(54)word in
+    // -2^20 <= xhi - pchi < 2^20
+    (word_uge xhi pchi /\ word_ult (word_sub xhi pchi) (word (2 EXP 20))) \/
+    (word_ult xhi pchi /\ word_ule (word_sub pchi xhi) (word (2 EXP 20)))`);;
+
+let ADRP_ADD_FOLD = prove(`forall (pc:int64) (x:int64).
+  adrp_within_bounds x pc
+  ==>
+  word_add
+    (word_add
+        (word_and pc (word 0xFFFFFFFFFFFFF000))
+        (word_sx
+            (word_join
+                (word_join
+                    (word_subword
+                        (word_sub
+                            (word_and x (word 0xFFFFFFFFFFFFF000))
+                            (word_and pc (word 0xFFFFFFFFFFFFF000)):(64)word)
+                        (14,19):(19)word)
+                    (word_subword
+                        (word_sub
+                            (word_and x (word 0xFFFFFFFFFFFFF000))
+                            (word_and pc (word 0xFFFFFFFFFFFFF000)):(64)word)
+                        (12,2):(2)word)
+                    :(21)word)
+                (word 0:(12)word)
+            :(33)word)
+        :(64)word)
+    )
+    (word (val (word_subword x (0,12):(12)word)):(64)word)
+    = x`,
+
+  REWRITE_TAC[adrp_within_bounds] THEN
+  BITBLAST_TAC);;
