arm/tutorial/symtab_rodata.ml
@@ -1,0 +1,136 @@
+(*
+ * Copyright Amazon.com, Inc. or its affiliates. All Rights Reserved.
+ * SPDX-License-Identifier: Apache-2.0 OR ISC OR MIT-0
+ *)
+
+(******************************************************************************
+          Verifying a program that reads constant data from .rodata
+******************************************************************************)
+
+needs "arm/proofs/base.ml";;
+
+(* The following command will print the assertion checker fn of
+   "arm/tutorial/symtab_rodata.o":
+
+   print_literal_relocs_from_elf "arm/tutorial/symtab_rodata.o";;
+*)
+
+let a_mc,a_constants_data = define_assert_relocs_from_elf "a_mc"
+    "arm/tutorial/symtab_rodata.o"
+(fun w BL ADR ADRP ADD_rri64 -> [
+  w 0xaa0003e3;         (* arm_MOV X3 X0 *)
+  ADRP (mk_var("x",`:num`),0,4,0);
+  ADD_rri64 (mk_var("x",`:num`),0,0,0);
+  w 0xaa0303e1;         (* arm_MOV X1 X3 *)
+  w 0xb8617801;         (* arm_LDR W1 X0 (Shiftreg_Offset X1 2) *)
+  ADRP (mk_var("y",`:num`),0,20,0);
+  ADD_rri64 (mk_var("y",`:num`),0,0,0);
+  w 0xaa0303e2;         (* arm_MOV X2 X3 *)
+  w 0xb8627800;         (* arm_LDR W0 X0 (Shiftreg_Offset X2 2) *)
+  w 0x0b000020;         (* arm_ADD W0 W1 W0 *)
+  w 0xd65f03c0          (* arm_RET X30 *)
+]);;
+
+(* Compared to the result of define_asserts_from_elf, the return value of
+    define_assert_relocs_from_elf has the following differences:
+    
+    1. It returns a_constants_data, which is a list of thm.
+      Each thm describes a definition of an object in a read-only section:
+      
+      # a_constants_data;;
+
+      - : thm list =
+      [|- y_data = [word 1; word 0; word 0; word 0; ...];
+       |- x_data = [word 2; word 0; word 0; word 0; ...]]
+
+    2. The returned a_mc is a function that takes the addresses of pc, x, y and
+       (x and y are the addresses of the two constant arrays) and returns
+       the corresponding machine code.
+
+      # a_mc;;
+
+      - : thm =
+      |- forall x pc y. b_mc pc x y = CONS (word 227) (...)
+*)
+
+let EXEC = ARM_MK_EXEC_RULE a_mc;;
+
+let A_SPEC = prove(`forall pc retpc x y i.
+  // These two assumptions state that the distance between symbol x and pc+4
+  // (which is the first adrp) do not overflow, and so does symbol y and
+  // pc+20.
+  adrp_within_bounds (word x) (word (pc + 4)) /\
+  adrp_within_bounds (word y) (word (pc + 20)) /\
+  i < 10
+  ==>
+  ensures arm
+    (\s. aligned_bytes_loaded s (word pc) (a_mc pc x y) /\
+         bytes_loaded s (word x) x_data /\
+         bytes_loaded s (word y) y_data /\
+         read PC s = word pc /\
+         read X0 s = word i /\
+         read X30 s = word retpc)
+    (\s. read W0 s = word (3 * (1 + i)) /\
+         read PC s = word retpc)
+    (MAYCHANGE [X0; X1; X2; X3; PC])`,
+
+  REPEAT STRIP_TAC THEN
+  ENSURES_INIT_TAC "s0" THEN
+
+  (* Let's prove the constant array is storing some structured int sequence. *)
+  SUBGOAL_THEN
+      `read (memory :> bytes32 (word_add (word x) (word (4 * i)))) s0 = word (2 * (i+1)) /\
+       read (memory :> bytes32 (word_add (word y) (word (4 * i)))) s0 = word (i+1)`
+      MP_TAC THENL [
+
+    (* Explode the 40-byte constant memory reads into 40 1-bytes!
+       Do it twice, one for x and one for y. *)
+    REPEAT_N 2 (
+      FIRST_X_ASSUM (fun th ->
+        (* Unfold the constant arrays! *)
+        let unfolded_bytes_loaded = REWRITE_RULE(bytes_loaded::a_constants_data) th in
+        (* Fold LENGTH array, and explode arr using BYTELIST_EXPAND_CONV *)
+        MP_TAC (CONV_RULE (ONCE_DEPTH_CONV LENGTH_CONV THENC
+                          LAND_CONV BYTELIST_EXPAND_CONV)
+                unfolded_bytes_loaded)) THEN
+      (* [a;b;..] = [x;y;..] is a = x /\ b = y /\ ... *)
+      REWRITE_TAC [CONS_11] THEN
+      STRIP_TAC) THEN
+
+    (* For each case where i < 10, concretely evaluate the values from the
+       exploded bytes, proving the equality. *)
+    UNDISCH_TAC `i < 10` THEN
+    SPEC_TAC (`i:num`,`i:num`) THEN
+    CONV_TAC EXPAND_CASES_CONV THEN
+
+    (* Convert the goal into word_joins of 1-byte reads as well. *)
+    REWRITE_TAC[READ_MEMORY_BYTESIZED_SPLIT] THEN
+    (* Offset canonicalization, and then rewrite using assumptions *)
+    REWRITE_TAC[WORD_ADD_ASSOC_CONSTS;WORD_ADD_0;ARITH] THEN
+    ASM_REWRITE_TAC[] THEN CONV_TAC WORD_REDUCE_CONV;
+
+    ALL_TAC
+  ] THEN
+
+  STRIP_TAC THEN
+  (* An extra equality that helps ARM_STEPS_TAC pick the right
+     memory read equation. "arm_print_log := true;;" will help you what
+     happens when this rule does not exist. *)
+  ASSUME_TAC (WORD_RULE `word (4 * val (word i:int64)):int64 = word (4 * i)`) THEN
+
+  REWRITE_TAC[ARITH] THEN
+  REPEAT STRIP_TAC THEN
+  ARM_STEPS_TAC EXEC (1--3) THEN
+  FIRST_X_ASSUM (fun th -> MP_TAC th THEN IMP_REWRITE_TAC[ADRP_ADD_FOLD] THEN DISCH_TAC) THEN
+
+  ARM_STEPS_TAC EXEC (4--7) THEN
+  FIRST_X_ASSUM (fun th -> MP_TAC th THEN IMP_REWRITE_TAC[ADRP_ADD_FOLD] THEN DISCH_TAC) THEN
+
+  ARM_STEPS_TAC EXEC (8--11) THEN
+
+  (* Prove the postcondition. *)
+  ENSURES_FINAL_STATE_TAC THEN
+
+  ASM_REWRITE_TAC[WREG_EXPAND_CLAUSES;READ_ZEROTOP_32] THEN
+  REWRITE_TAC[WORD_BLAST`word_zx (word_zx (x:(32)word):(64)word):(32)word = x`] THEN
+  CONV_TAC WORD_RULE);;
